Let us unroll the definition of subset relation\footnote{
$X \subseteq Y \quad \defsign \quad \forall x.\ (x \in X \implies x \in Y)$.}
in the definition of semantic subtyping:
\begin{equation}
\bjtruesemsub{\ty_1}{\ty_2} \quad \defsign \quad
\forall \vty.\ (\vty \in \interpty{\ty_1} \implies \vty \in \interpty{\ty_2}).
\end{equation}
Its main ingredient is in-the-interpretation relation $\vty \in \interpty{\ty}$.
We can define an inductive syntax-directed relation
equivalent to $\vty \in \interpty{\ty}$.
We call this relation \defemph{matching relation} 
and denote by $\bjmtch{\vty}{\ty}$, 
read ``value type \vty matches \ty''.
The formal definition is given in~\figref{fig:bjsem-match}.
The matching and in-the-interpretation relations are equivalent:
\begin{equation}\label{eq:match-eq-in-the-interpty}
\forall \vty.\ (\vty \in \interpty{\ty} \quad \iff \quad \bjmtch{\vty}{\ty}).
\end{equation}
The proof is done by induction on \ty (\appref{app:match}).

\begin{figure}
	\begin{mathpar}
		\inferrule*[right=MT-CName]
		{ }
		{ \bjmtch{\cname}{\cname} }		
		\\
		
		\inferrule*[right=\footnotesize{MT-IntReal}]
		{ }
		{ \bjmtch{\tyint}{\tyreal} }
		
		\inferrule*[right=\footnotesize{MT-FltReal}]
		{ }
		{ \bjmtch{\tyflt}{\tyreal} }
		\\
		
		\inferrule*[right=MT-IntNum]
		{ }
		{ \bjmtch{\tyint}{\tynum} }
		
		\inferrule*[right=MT-FltNum]
		{ }
		{ \bjmtch{\tyflt}{\tynum} }
		
		\inferrule*[right=MT-CmplxNum]
		{ }
		{ \bjmtch{\tycmplx}{\tynum} }
		\\
		
		\inferrule*[right=MT-Pair]
		{ \bjmtch{\vty_1}{\ty_1} \\ \bjmtch{\vty_2}{\ty_2} }
		{ \bjmtch{\typair{\vty_1}{\vty_2}}{\typair{\ty_1}{\ty_2}} }
		\\
		
		\inferrule*[right=MT-Union1]
		{ \bjmtch{\vty}{\ty_1}  }
		{ \bjmtch{\vty}{\tyunion{\ty_1}{\ty_2}} }
		
		\inferrule*[right=MT-Union2]
		{ \bjmtch{\vty}{\ty_2}  }
		{ \bjmtch{\vty}{\tyunion{\ty_1}{\ty_2}} }
	\end{mathpar}
	\caption{Matching Relation in \BetaJulia}
	\label{fig:bjsem-match}
\end{figure}

Using the matching relation, we define a \emph{syntactic model} of
semantic subtyping as follows:
\begin{equation}
\bjsemsub{\ty_1}{\ty_2} \quad \defsign \quad
\forall \vty.\ (\bjmtch{\vty}{\ty_1} \implies \bjmtch{\vty}{\ty_1}).
\end{equation}
By~\ref{eq:match-eq-in-the-interpty}, we have that $\bjsemsub{\ty_1}{\ty_2}$
is equivalent to our definition of semantic subtyping for \BetaJulia:
\begin{equation}
\bjsemsub{\ty_1}{\ty_2} \quad \iff \quad \bjtruesemsub{\ty_1}{\ty_2}.
\end{equation}
We will be using